\documentclass[12pt]{article}

%%% UPDATE THESE PARAMETERS
\newcommand{\sid}{530157791}
\newcommand{\assignment}{2}
\newcommand{\uos}{comp2022}
%%%

\NeedsTeXFormat{LaTeX2e}
\usepackage[osf]{mathpazo}
\usepackage[svgnames]{xcolor}
\usepackage[T1]{fontenc}
\usepackage{amsmath,amsthm,amsfonts,amssymb,mathtools}
\usepackage{hyperref,url}
\usepackage[margin=2.7cm,a4paper]{geometry}
\usepackage{tasks}
\usepackage{xstring}
\usepackage[tikz]{mdframed}
\usepackage{environ}
\usepackage{etoolbox}
\usepackage{fourier-orns}
\usepackage{kvoptions}
\usepackage[]{units}
\usepackage{url}%
\usepackage[normal]{subfigure}

% math config

\DeclarePairedDelimiter\ceil{\lceil}{\rceil}
\DeclarePairedDelimiter\abs{\lvert}{\rvert}
\DeclarePairedDelimiter\set{\{}{\}}


% headers

\usepackage{fancyhdr}
\addtolength{\headheight}{2.5pt}
\pagestyle{fancy}
\fancyhead{} 
\fancyhead[L]{\sc \uos} 
\renewcommand{\headrulewidth}{0.75pt}

% update these headers
\fancyhead[C]{\sc SID: \sid}
\fancyhead[R]{Assignment \assignment}


% pseudo-code typesetting configuration
\usepackage[tikz]{mdframed}
\usepackage[noend]{algpseudocode}

\newenvironment{pseudocode}
{
  \mdframed
  \algorithmic[1]
}
{
  \endalgorithmic
  \endmdframed
}

% solution 

\newcommand{\solution}[1]{\noindent \textbf{Solution #1.}}


\begin{document}

\solution{4}
To replace rules forms $AB \rightarrow c$, we need to know how \( AB \) can be derived. Below are all the cases in which \( AB \) can be derived. 

\begin{enumerate}

  \item For each rule of the form \( U \rightarrow AB \), replace \( AB \) on the right-hand side with \( c \), and introduce a new rule \( U \rightarrow c \).

  \item If a rule \( Z \rightarrow XC \) exists, where \( X \rightarrow YA \) (with the string ending in \( A \)) and \( C \rightarrow BD \) (with the string starting with \( B \)), introduce a new rule \( Z \rightarrow YcD \).

  For every rule in the form \( X \rightarrow YA \), if there is a rule \( E \rightarrow XB \), add a new rule \( E \rightarrow Yc \).


  \item For every rule in the form of \( P \rightarrow AQ \), if we want to derive \( AB \), then \( Q \) needs to derive something that starts with \( B \) during the derivation process. For each derivation that starts with \( B \) (i.e., \( B \) followed by remaining variables or terminal symbols \( R \)), we add a new rule \( G \rightarrow cR \).
\end{enumerate}


By adding these new rules to replace \( AB \rightarrow c \), we can remove the rule \( AB \rightarrow c \). The new context-free grammar will be equivalent to the original one.

\end{document}
